resolve sorrys in ViperBoogieEndToEnd

ViperBoogieEndToEnd.thy
@@ -7,12 +7,6 @@ definition stmt_correct_total_2 where
         \<forall>(\<omega> :: 'a full_total_state) r. is_empty_total \<omega> \<longrightarrow> 
                   red_stmt_total ctxt R \<Lambda> s \<omega> r \<longrightarrow> r \<noteq> RFailure"
 
-term red_cfg
-
-term stmt_rel
-
-typ "'a vbpl_absval"
-
 lemma proc_is_correct_elim:
   assumes 
      "proc_is_correct A fun_decls constants global_vars axioms proc proc_body_satisfies_spec_general" and
@@ -39,38 +33,131 @@ lemma valid_configuration_not_failure:
   unfolding valid_configuration_def
   by simp
 
-(*
-declare [[show_types]]
-declare [[show_sorts]]
-declare [[show_consts]]
-*)
-
 type_synonym ('a,'m) proc_body_satisfies_spec_ty = 
    "'a absval_ty_fun \<Rightarrow> 'm proc_context \<Rightarrow> var_context \<Rightarrow> 'a fun_interp \<Rightarrow> rtype_env \<Rightarrow> expr list \<Rightarrow> expr list \<Rightarrow> ast \<Rightarrow> 'a nstate \<Rightarrow> bool"
 
 abbreviation state_rel_initial where 
-  "state_rel_initial ctxt Pr ty_rep tr_vpr_bpl wd_mask w ns \<equiv> 
-       state_rel Pr ty_rep tr_vpr_bpl ctxt wd_mask w w ns"
+  "state_rel_initial ctxt Pr TyRep Tr AuxPred w ns \<equiv> 
+       state_rel Pr TyRep Tr AuxPred ctxt w w ns"
 
 abbreviation red_bigblock_multi where
   "red_bigblock_multi A M \<Lambda> \<Gamma> \<Omega> ast \<equiv> rtranclp (red_bigblock A M \<Lambda> \<Gamma> \<Omega> ast)"
 
-(*
-      "\<lbrakk> (type_interp ctxt), ([] :: ast proc_context), (var_context ctxt), (fun_interp ctxt), [] \<turnstile> \<langle>c, s\<rangle> \<rightarrow> s' \<rbrakk> \<Longrightarrow>
-       red_bigblock_small P ctxt (((BigBlock name (c#cs) str tr), cont), s) (((BigBlock name cs str tr), cont), s')"
-*)
-lemma test:
-  assumes RedSingleCmd: "A, M, \<Lambda>, \<Gamma>, \<Omega> \<turnstile> \<langle>c, s\<rangle> \<rightarrow> s'" and
-          Red: "red_bigblock_multi A M \<Lambda> \<Gamma> \<Omega> ast (BigBlock name cs str tr, cont, s') c'"
-  shows "red_bigblock_multi A M \<Lambda> \<Gamma> \<Omega> ast (BigBlock name (c#cs) str tr, cont, s) c'"
-  sorry
-  
+lemma magic_stays_red_bigblock:
+  assumes " A,M,\<Lambda>,\<Gamma>,\<Omega>,ast \<turnstile> \<langle>y\<rangle> \<longrightarrow> z" and
+         "snd (snd y) = Magic"
+       shows  "snd (snd z) = Magic"
+  using assms
+  by (cases) auto
+
+lemma magic_stays_red_bigblock_multi:
+   assumes "red_bigblock_multi A M \<Lambda> \<Gamma> \<Omega> ast \<gamma> \<gamma>'" and
+      "snd (snd \<gamma>) = Magic"
+    shows "snd (snd \<gamma>') = Magic"
+  using assms 
+  apply induction
+   apply simp
+  using magic_stays_red_bigblock
+  by blast  
+
+inductive_cases RedSimpleCmdsCons_case: "A,M,\<Lambda>,\<Gamma>,\<Omega>,T \<turnstile> \<langle>((BigBlock bb_name (c#cs) str_cmd tr_cmd), cont0, Normal n_s)\<rangle> \<longrightarrow> y"
+
+lemma red_bigblock_multi_simple_cmds_cons_failure:
+  assumes 
+          RedMulti: "red_bigblock_multi A M \<Lambda> \<Gamma> \<Omega> ast \<gamma> \<gamma>'" and
+               "\<gamma> = (BigBlock name cs str tr, cont, s')" and
+          RedSingleCmd: "A, M, \<Lambda>, \<Gamma>, \<Omega> \<turnstile> \<langle>c, s\<rangle> \<rightarrow> s'" and
+          FailureConfig:   "snd (snd \<gamma>') = Failure"
+             shows "\<exists> \<gamma>'. red_bigblock_multi A M \<Lambda> \<Gamma> \<Omega> ast (BigBlock name (c#cs) str tr, cont, s) \<gamma>' \<and> snd (snd \<gamma>') = Failure"
+proof (cases s')
+  case (Normal ns)
+  hence "A,M,\<Lambda>,\<Gamma>,\<Omega> \<turnstile> \<langle>c,s\<rangle> \<rightarrow> Normal ns"
+    using RedSingleCmd
+    by simp
+  from this obtain ns0 where "s = Normal ns0"
+    by (cases) (assumption+)
+
+  from RedMulti have RedMulti2: "red_bigblock_multi A M \<Lambda> \<Gamma> \<Omega> ast (BigBlock name cs str tr, cont, Normal ns) \<gamma>'"
+    using \<open>\<gamma> = _\<close> \<open>s' = _\<close>
+    by blast
+
+  from this
+  obtain s'' where "A, M, \<Lambda>, \<Gamma>, \<Omega> \<turnstile> \<langle>cs, Normal ns\<rangle> [\<rightarrow>] s''" and 
+                   RedMultiEmptySimpleCmds: "red_bigblock_multi A M \<Lambda> \<Gamma> \<Omega> ast (BigBlock name [] str tr, cont, s'') \<gamma>'"
+  proof -
+    assume *: "(\<And>s''. A,M,\<Lambda>,\<Gamma>,\<Omega> \<turnstile> \<langle>cs,Normal ns\<rangle> [\<rightarrow>] s'' \<Longrightarrow>
+            red_bigblock_multi A M \<Lambda> \<Gamma> \<Omega> ast (BigBlock name [] str tr, cont, s'') \<gamma>' \<Longrightarrow> thesis)"
+    show ?thesis
+    proof (cases cs)
+      case Nil
+      thus ?thesis
+        using * RedMulti2 RedCmdListNil by blast
+    next
+      case (Cons c' cs')
+
+      from RedMulti2 \<open>cs = _\<close> obtain s'' where "A, M, \<Lambda>, \<Gamma>, \<Omega> \<turnstile> \<langle>cs, Normal ns\<rangle> [\<rightarrow>] s''" and
+                                      "red_bigblock_multi A M \<Lambda> \<Gamma> \<Omega> ast (BigBlock name [] str tr, cont, s'') \<gamma>'"
+        apply (cases rule: converse_rtranclpE)
+        using FailureConfig
+         apply fastforce
+        using RedSimpleCmdsCons_case
+        by metis
+
+      then show ?thesis 
+        using * by simp
+    qed
+  qed
+
+  hence RedList: "A, M, \<Lambda>, \<Gamma>, \<Omega> \<turnstile> \<langle>c#cs, s\<rangle> [\<rightarrow>] s''"
+    using RedSingleCmd \<open>s' = _\<close>
+    by (auto intro: RedCmdListCons)
+
+  show ?thesis     
+    apply (rule exI, rule conjI)
+     apply (rule converse_rtranclp_into_rtranclp)
+    apply (subst \<open>s = _\<close>)
+      apply (rule RedSimpleCmds)
+    using RedList RedMultiEmptySimpleCmds \<open>s = _\<close> FailureConfig
+    by auto        
+next
+  case Failure
+  hence RedListFailure: "A, M, \<Lambda>, \<Gamma>, \<Omega> \<turnstile> \<langle>c#cs, s\<rangle> [\<rightarrow>] Failure"
+    using RedSingleCmd
+    by (simp add: RedCmdListCons failure_red_cmd_list)
+  show ?thesis
+  proof (cases s)
+    case (Normal ns)
+    show ?thesis 
+      apply (subst Normal)
+      apply (rule exI, rule conjI)
+       apply (rule converse_rtranclp_into_rtranclp)
+        apply (rule RedSimpleCmds)
+      using RedListFailure Normal
+      by auto            
+  next
+    case Failure
+    then show ?thesis 
+      by auto
+  next
+    case Magic
+    \<comment>\<open>cannot occur\<close>
+    with RedListFailure show ?thesis
+      using magic_stays_cmd_list by blast
+  qed
+next
+  case Magic
+  \<comment>\<open>cannot occur\<close>
+  then show ?thesis 
+    using magic_stays_red_bigblock_multi assms
+    by (metis RedMulti sndI state.distinct(5))
+qed
 
 lemma red_ast_block_red_bigblock_failure_preserve:
   assumes "red_ast_bpl P ctxt c c'" and 
-          "snd c = Normal ns" and
           "snd c' = Failure" and 
-          "type_interp ctxt = A" and "var_context ctxt = \<Lambda>" and "fun_interp ctxt = \<Gamma>"
+          "type_interp ctxt = A" and 
+          "var_context ctxt = \<Lambda>" and 
+          "fun_interp ctxt = \<Gamma>"
         shows "\<exists>d'. red_bigblock_multi A ([] :: ast proc_context) \<Lambda> \<Gamma> [] P (fst (fst c), snd (fst c), snd c) d' 
                     \<and> (snd (snd d') = Failure)"
   using assms
@@ -83,18 +170,17 @@ next
   from this obtain d' where    
      Red2: "red_bigblock_multi A ([] :: ast proc_context) \<Lambda> \<Gamma> [] P (fst (fst z), snd (fst z), snd z) d'" and
      Red2StateFailure: "snd (snd d') = Failure"
-    by blast  
+    by blast
 
   from \<open>red_bigblock_small P ctxt y z\<close>
   show ?case
   proof cases
     case (RedBigBlockSmallSimpleCmd c s s' name cs str tr cont)
-    have "red_bigblock_multi (type_interp ctxt) ([] :: ast proc_context) (var_context ctxt) (fun_interp ctxt) [] P (BigBlock name (c # cs) str tr, cont, s) d'"
-      apply (rule test)
-      using RedBigBlockSmallSimpleCmd
-      apply simp
-      using Red2 \<open>z = _\<close> assms
-      by simp
+    from this obtain \<gamma>' where
+    "red_bigblock_multi (type_interp ctxt) ([] :: ast proc_context) (var_context ctxt) (fun_interp ctxt) [] P (BigBlock name (c # cs) str tr, cont, s) \<gamma>' \<and>
+     (snd (snd \<gamma>')) = Failure"
+      using red_bigblock_multi_simple_cmds_cons_failure RedBigBlockSmallSimpleCmd Red2
+      by (metis Red2StateFailure assms(3) assms(5) prod.collapse prod.inject step.prems(3))
     thus ?thesis
       using Red2StateFailure \<open>y = _\<close> assms
       by fastforce
@@ -107,7 +193,7 @@ next
 qed
 
 lemma init_ast_convert_ast_to_program_point_eq:
-  "(init_ast ast ns) =  (fst (convert_ast_to_program_point ast), snd (convert_ast_to_program_point ast),
+  "(init_ast ast ns) = (fst (convert_ast_to_program_point ast), snd (convert_ast_to_program_point ast),
          Normal ns)"
   by (cases ast) auto
 
@@ -120,7 +206,6 @@ lemma proc_body_satisfies_spec_valid_config:
   unfolding proc_body_satisfies_spec_def
   by blast
 
-
 lemma end_to_end_stmt_rel:
   assumes ProcBodySome: "proc_body proc_bpl = Some (locals_bpl, proc_body_bpl)" and
 
@@ -128,15 +213,14 @@ lemma end_to_end_stmt_rel:
           ProcPresEmpty: "proc_pres proc_bpl = []" and
           \<comment>\<open>The Boogie procedure is correct.\<close>             
              \<comment>\<open>Note that we need to explicitly provide the type for term\<open>A\<close> to 
-                be able to instantiate A with \<^term>\<open>vbpl_absval_ty ty_rep\<close>\<close>
+                be able to instantiate A with \<^term>\<open>vbpl_absval_ty TyRep\<close>\<close>
           Boogie_correct: "\<And>A :: ('a vbpl_absval) absval_ty_fun. proc_is_correct A fun_decls constants global_vars axioms (proc_bpl :: ast procedure) 
-                  (Ast.proc_body_satisfies_spec :: (('a vbpl_absval, ast) proc_body_satisfies_spec_ty))" and          
-
+                  (Ast.proc_body_satisfies_spec :: (('a vbpl_absval, ast) proc_body_satisfies_spec_ty))" and
 
           \<comment>\<open>Viper and Boogie statement are related\<close>
           StmtRel: "stmt_rel 
              \<comment>\<open>input relation\<close>
-             (state_rel_empty (state_rel_initial ctxt Pr (ty_rep :: 'a ty_repr_bpl) tr_vpr_bpl (mask_var tr_vpr_bpl)))
+             (state_rel_empty (state_rel_initial ctxt Pr (TyRep :: 'a ty_repr_bpl) Tr AuxPred))
              \<comment>\<open>output relation is irrelevant\<close>
              R' 
              ctxt_vpr StateCons \<Lambda> proc_body_bpl ctxt 
@@ -145,19 +229,19 @@ lemma end_to_end_stmt_rel:
              (convert_ast_to_program_point proc_body_bpl)
              \<comment>\<open>output program point in Boogie procedure body is irrelevant\<close>
              \<gamma>'"  and 
-    TypeInterpEq: "type_interp ctxt = (vbpl_absval_ty ty_rep)" and
+    TypeInterpEq: "type_interp ctxt = (vbpl_absval_ty TyRep)" and
     ProcTyArgsEmpty: "proc_ty_args proc_bpl = 0" and
     VarCtxtEq: "var_context ctxt = (constants @ global_vars, proc_args proc_bpl @ locals_bpl @ proc_rets proc_bpl)" and
 \<comment>\<open>TODO: I have not yet proved the following assumptions for specific Boogie programs\<close>
-     WfTyRep: "wf_ty_repr_bpl ty_rep" and
-     FunInterp: "fun_interp_wf (vbpl_absval_ty ty_rep) fun_decls (fun_interp ctxt)" and
+     WfTyRep: "wf_ty_repr_bpl TyRep" and
+     FunInterp: "fun_interp_wf (vbpl_absval_ty TyRep) fun_decls (fun_interp ctxt)" and
      InitialStateRel: "\<And> \<omega>. is_empty_total \<omega> \<Longrightarrow> 
                        \<exists>ns ls gs.
                            ns = \<lparr>old_global_state = gs, global_state = gs, local_state = ls, binder_state = Map.empty\<rparr> \<and>  
-                           (state_rel_empty (state_rel_initial ctxt Pr (ty_rep :: 'a ty_repr_bpl) tr_vpr_bpl (mask_var tr_vpr_bpl))) \<omega> ns \<and>
-                           state_typ_wf (vbpl_absval_ty ty_rep) [] gs (constants @ global_vars) \<and>
-                           state_typ_wf (vbpl_absval_ty ty_rep) [] ls ((proc_args proc_bpl)@ (locals_bpl @ proc_rets proc_bpl)) \<and>
-                           axioms_sat (vbpl_absval_ty ty_rep) (constants, []) (fun_interp ctxt) (global_to_nstate (state_restriction gs constants)) axioms"
+                           (state_rel_empty (state_rel_initial ctxt Pr (TyRep :: 'a ty_repr_bpl) Tr AuxPred)) \<omega> ns \<and>
+                           state_typ_wf (vbpl_absval_ty TyRep) [] gs (constants @ global_vars) \<and>
+                           state_typ_wf (vbpl_absval_ty TyRep) [] ls ((proc_args proc_bpl)@ (locals_bpl @ proc_rets proc_bpl)) \<and>
+                           axioms_sat (vbpl_absval_ty TyRep) (constants, []) (fun_interp ctxt) (global_to_nstate (state_restriction gs constants)) axioms"
 
   shows "stmt_correct_total_2 ctxt_vpr StateCons \<Lambda> stmt_vpr"
   unfolding stmt_correct_total_2_def
@@ -165,35 +249,36 @@ proof (rule allI | rule impI)+
   fix \<omega> r 
   assume "is_empty_total \<omega>" and RedStmtVpr:"red_stmt_total ctxt_vpr StateCons \<Lambda> stmt_vpr \<omega> r"
   
-  let ?abs="vbpl_absval_ty ty_rep"
+  let ?abs="vbpl_absval_ty TyRep"
 
   note Boogie_correct_inst=Boogie_correct[where ?A="?abs"]
 
   obtain ns ls gs where 
     "ns = \<lparr>old_global_state = gs, global_state = gs, local_state = ls, binder_state = Map.empty\<rparr>" and
   StmtRelInitialInst: 
-    "(state_rel_empty (state_rel_initial ctxt Pr (ty_rep :: 'a ty_repr_bpl) tr_vpr_bpl (mask_var tr_vpr_bpl))) \<omega> ns" and
+    "state_rel_empty (state_rel_initial ctxt Pr (TyRep :: 'a ty_repr_bpl) Tr AuxPred) \<omega> ns" and
   GlobalsWf:
-    "state_typ_wf (vbpl_absval_ty ty_rep) [] gs (constants @ global_vars)" and
+    "state_typ_wf (vbpl_absval_ty TyRep) [] gs (constants @ global_vars)" and
   LocalsWf:
-    "state_typ_wf (vbpl_absval_ty ty_rep) [] ls ((proc_args proc_bpl)@ (locals_bpl @ proc_rets proc_bpl))" and
+    "state_typ_wf (vbpl_absval_ty TyRep) [] ls ((proc_args proc_bpl)@ (locals_bpl @ proc_rets proc_bpl))" and
   AxiomsSat:
-    "axioms_sat (vbpl_absval_ty ty_rep) (constants, []) (fun_interp ctxt) (global_to_nstate (state_restriction gs constants)) axioms"
+    "axioms_sat (vbpl_absval_ty TyRep) (constants, []) (fun_interp ctxt) (global_to_nstate (state_restriction gs constants)) axioms"
     using InitialStateRel[OF \<open>is_empty_total \<omega>\<close>]
     by blast
+    
   
   have ProcBodyBplCorrect:
       "(Ast.proc_body_satisfies_spec :: (('a vbpl_absval, ast) proc_body_satisfies_spec_ty)) ?abs [] (constants@global_vars, (proc_args proc_bpl)@(locals_bpl@(proc_rets proc_bpl))) (fun_interp ctxt) [] 
                                        (proc_all_pres proc_bpl) (proc_checked_posts proc_bpl) proc_body_bpl
                                        \<lparr>old_global_state = gs, global_state = gs, local_state = ls, binder_state = Map.empty\<rparr>"
   proof (rule proc_is_correct_elim[OF Boogie_correct_inst ProcBodySome])
-    show "\<forall>t. closed t \<longrightarrow> (\<exists>v. type_of_vbpl_val ty_rep v = t)"
+    show "\<forall>t. closed t \<longrightarrow> (\<exists>v. type_of_vbpl_val TyRep v = t)"
       by (simp add: closed_types_inhabited)
   next
-    show "\<forall>v. closed (type_of_vbpl_val ty_rep v)"
+    show "\<forall>v. closed (type_of_vbpl_val TyRep v)"
     proof (rule allI)
       fix v
-      show "closed (type_of_vbpl_val ty_rep v)"
+      show "closed (type_of_vbpl_val TyRep v)"
       proof (cases v)
         case (LitV x1)
         then show ?thesis by simp
@@ -205,19 +290,19 @@ proof (rule allI | rule impI)+
       qed
     qed
   next
-    show "fun_interp_wf (vbpl_absval_ty ty_rep) fun_decls (fun_interp ctxt)"
+    show "fun_interp_wf (vbpl_absval_ty TyRep) fun_decls (fun_interp ctxt)"
       by (rule FunInterp)
   next
     show "list_all closed [] \<and> length []  = proc_ty_args proc_bpl"
       by (simp add: ProcTyArgsEmpty)
   next
-    show "state_typ_wf (vbpl_absval_ty ty_rep) [] gs (constants @ global_vars)"
+    show "state_typ_wf (vbpl_absval_ty TyRep) [] gs (constants @ global_vars)"
       by (rule GlobalsWf)
   next 
-    show "state_typ_wf (vbpl_absval_ty ty_rep) [] ls (proc_args proc_bpl @ locals_bpl @ proc_rets proc_bpl)"
+    show "state_typ_wf (vbpl_absval_ty TyRep) [] ls (proc_args proc_bpl @ locals_bpl @ proc_rets proc_bpl)"
       by (rule LocalsWf)
   next
-    show "axioms_sat (vbpl_absval_ty ty_rep) (constants, []) (fun_interp ctxt) (global_to_nstate (state_restriction gs constants)) axioms"
+    show "axioms_sat (vbpl_absval_ty TyRep) (constants, []) (fun_interp ctxt) (global_to_nstate (state_restriction gs constants)) axioms"
       by (rule AxiomsSat)
   qed
 
@@ -235,16 +320,11 @@ proof (rule allI | rule impI)+
     let ?c'_bigblock = "fst ?c'_program_point"
     let ?c'_cont = "snd ?c'_program_point"
 
-    thm red_ast_block_red_bigblock_failure_preserve[OF RedBpl FailureConfig TypeInterpEq VarCtxtEq HOL.refl]
-    thm RedBpl
-
     obtain d' where 
-      RedBigBlockMulti: "(red_bigblock_multi (vbpl_absval_ty ty_rep) ([] :: ast proc_context) (constants @ global_vars, proc_args proc_bpl @ locals_bpl @ proc_rets proc_bpl) (fun_interp ctxt) [] proc_body_bpl)\<^sup>*\<^sup>*
+      RedBigBlockMulti: "(red_bigblock_multi (vbpl_absval_ty TyRep) ([] :: ast proc_context) (constants @ global_vars, proc_args proc_bpl @ locals_bpl @ proc_rets proc_bpl) (fun_interp ctxt) [] proc_body_bpl)\<^sup>*\<^sup>*
          (init_ast proc_body_bpl \<lparr>old_global_state = gs, global_state = gs, local_state = ls, binder_state = Map.empty\<rparr>) d'" and
       "snd (snd d') = Failure"
-   \<comment>\<open>TODO: need to prove that if Boogie program reduces to Failure with red_ast_bpl, then this must also be the case with
-           red_bigblock (difference is that red_ast_bpl reduces simple command by simple command, while red_bigblock reduces
-           all the simple commands at once)\<close>
+
       using red_ast_block_red_bigblock_failure_preserve[OF RedBpl FailureConfig TypeInterpEq VarCtxtEq HOL.refl]
             \<open>ns = _\<close>      
       by (auto simp: init_ast_convert_ast_to_program_point_eq)
@@ -253,7 +333,7 @@ proof (rule allI | rule impI)+
     let ?d'_cont = "fst (snd d')"
     let ?d'_state = "snd (snd d')"
 
-    have "Ast.valid_configuration (vbpl_absval_ty ty_rep) (constants @ global_vars, proc_args proc_bpl @ locals_bpl @ proc_rets proc_bpl)
+    have "Ast.valid_configuration (vbpl_absval_ty TyRep) (constants @ global_vars, proc_args proc_bpl @ locals_bpl @ proc_rets proc_bpl)
          (fun_interp ctxt) [] (Ast.proc_checked_posts proc_bpl) ?d'_bigblock ?d'_cont ?d'_state"
       apply (rule proc_body_satisfies_spec_valid_config[OF ProcBodyBplCorrect] )
       using ProcPresEmpty RedBigBlockMulti
